formal/examples/Drinks_Machine_2.thy
@@ -12,13 +12,13 @@ definition vend_nothing :: "transition" where
         Arity = 0,
         Guard = [],
         Outputs =  [],
-        Updates = [(R 1, V (R 1)), (R 2, V (R 2))]
+        Updates = [(1, V (R 1)), (2, V (R 2))]
       \<rparr>"
 
 lemma guard_vend_nothing: "Guard vend_nothing = []"
   by (simp add: vend_nothing_def)
 
-lemma updates_vend_nothing: "Updates vend_nothing = [(R 1, V (R 1)), (R 2, V (R 2))]"
+lemma updates_vend_nothing: "Updates vend_nothing = [(1, V (R 1)), (2, V (R 2))]"
   by (simp add: vend_nothing_def)
 
 lemmas transitions = Drinks_Machine.transitions vend_nothing_def
@@ -54,145 +54,45 @@ lemma possible_steps_2_coin: "length i = 1 \<Longrightarrow> possible_steps drin
   apply (simp add: possible_steps_def drinks2_def transitions)
   by force
 
-lemma possible_steps_2_vend: "r (R 2) = Some (Num n) \<Longrightarrow> n \<ge> 100 \<Longrightarrow> possible_steps drinks2 2 r ((STR ''vend'')) [] = {|(3, vend)|}"
-proof-
-  assume prem1: "r (R 2) = Some (Num n)"
-  assume prem2: "n \<ge> 100"
-  have filter: "ffilter
-     (\<lambda>((origin, dest), t).
-         origin = 2 \<and>
-         Label t = STR ''vend'' \<and> Arity t = 0 \<and> apply_guards (Guard t) (\<lambda>x. case x of I n \<Rightarrow> input2state [] 1 (I n) | R n \<Rightarrow> r (R n)))
-     drinks2 =
-    {|((2, 3), vend)|}"
-    apply (simp add: ffilter_def fset_both_sides Abs_fset_inverse drinks2_def Set.filter_def)
-    apply safe
-    using prem1 prem2
-    by (simp_all add: transitions gval.simps ValueGt_def)
-  show ?thesis
-    by (simp add: possible_steps_def filter)
-qed
+lemma possible_steps_2_vend: "r 2 = Some (Num n) \<Longrightarrow> n \<ge> 100 \<Longrightarrow> possible_steps drinks2 2 r ((STR ''vend'')) [] = {|(3, vend)|}"
+  apply (simp add: possible_steps_singleton drinks2_def)
+  apply safe
+  by (simp_all add: transitions apply_guards_def ValueGt_def)
 
 lemma purchase_coke: "observe_trace drinks2 0 <> [((STR ''select''), [Str ''coke'']), ((STR ''coin''), [Num 50]), ((STR ''coin''), [Num 50]), ((STR ''vend''), [])] =
                        [[], [Some (Num 50)], [Some (Num 100)], [Some (Str ''coke'')]]"
-  apply (simp add: observe_trace_def step_def possible_steps_0 updates_select)
-  apply (simp add: possible_steps_1 step_def updates_coin)
-  apply (simp add: possible_steps_2_coin step_def updates_coin)
-  using possible_steps_2_vend
-  apply simp
-  by (simp add: transitions )
-
-lemma "consistent (medial empty (Guard select))"
-  by (simp add: select_def medial_empty)
-
-definition r1_r2_true :: "context" where
-"r1_r2_true \<equiv> \<lbrakk>(V (R 1)) \<mapsto> {|Bc True|}, (V (R 2)) \<mapsto> {|Bc True|}\<rbrakk>"
-
-lemma posterior_coin_first: "posterior select_posterior coin = r1_r2_true"
-  apply (simp add: posterior_def posterior_separate_def coin_def medial_empty consistent_select_posterior)
-  apply (simp add: remove_obsolete_constraints_def r1_r2_true_def)
-  apply (rule ext)
-  by (simp add: select_posterior_def fprod_singletons)
-
-lemma consistent_r1_r2_true: "consistent r1_r2_true"
-  apply (simp add: consistent_def r1_r2_true_def cval_true)
-  using consistent_def consistent_empty by blast
-
-lemma posterior_coin_subsequent: "posterior r1_r2_true coin = r1_r2_true"
-  apply (simp add: posterior_def coin_def posterior_separate_def medial_empty consistent_r1_r2_true)
-  apply (simp add: remove_obsolete_constraints_def r1_r2_true_def)
-  apply (rule ext)
-  by (simp add: fprod_singletons r1_r2_true_def)
-
-lemma can_take_coin: "consistent c \<longrightarrow> Contexts.can_take coin c"
-  by (simp add: can_take_def coin_def medial_empty)
-
-lemma posterior_n_coin_true_true: "(posterior_n n coin r1_r2_true) = r1_r2_true"
-  proof (induct n)
-    case 0
-    then show ?case by simp
-  next
-    case (Suc n)
-    then show ?case
-      by (simp add: posterior_coin_subsequent)
-  qed
-
-lemma consistent_posterior_n_coin: "consistent (posterior_n n coin select_posterior)" (* We can go round coin as many times as we like *)
-  proof(induct n)
-    case 0
-    then show ?case
-      apply (simp add: consistent_def)
-      apply (simp add: select_posterior_def)
-      apply (rule_tac x="<R 2 := Num 0>" in exI)
-      apply (simp add: cval_def gval.simps ValueEq_def)
-      apply (rule allI)
-      apply (case_tac r)
-         apply (simp add: gval.simps)
-        apply (case_tac x2)
-         apply (simp add: gval.simps)
-        apply (simp add: gval.simps ValueEq_def)
-      by (simp_all add: gval.simps)
-  next
-    case (Suc n)
-    then show ?case
-      apply (simp add: posterior_coin_first posterior_n_coin_true_true)
-      using consistent_r1_r2_true r1_r2_true_def posterior_n_coin_true_true by auto
-  qed
-
-lemma posterior_n_coin_true_2: "(posterior_n (Suc n) coin select_posterior) = r1_r2_true"
-  proof (induction n)
-    case 0
-    then show ?case
-      apply (simp )
-      by (simp only: posterior_coin_first)
-  next
-    case (Suc n)
-    then show ?case
-      apply simp
-      apply (simp add: posterior_coin_first)
-      by (simp only: posterior_coin_subsequent)
-  qed
-
-lemma can_take_vend: "0 < Suc n \<longrightarrow> Contexts.can_take vend r1_r2_true"
-  apply (simp add: can_take_def vend_def medial_def r1_r2_true_def List.maps_def pairs2context_def consistent_def)
-  apply (rule_tac x="<R 2 := Num 100>" in exI)
-  apply (simp add: cval_def gval.simps ValueGt_def)
-  apply (rule allI)
-  apply (case_tac r)
-     apply (simp add: gval.simps)
-    apply (case_tac x2)
-     apply (simp add: gval.simps)
-    apply (simp add: gval.simps ValueEq_def)
-  by (simp_all add: gval.simps)
-
-lemma medial_vend: "medial r1_r2_true (Guard vend) = \<lbrakk>(V (R 1)) \<mapsto> {|Bc True|}, (V (R 2)) \<mapsto> {|Geq (Num 100), Bc True|}\<rbrakk>"
-  apply (rule ext)
-  by (simp add: vend_def r1_r2_true_def medial_def List.maps_def pairs2context_def)
-
-lemma consistent_medial_vend: "consistent (medial r1_r2_true (Guard vend))"
-  apply (simp add: consistent_def medial_vend)
-  apply (rule_tac x="<R 2 := Num 100>" in exI)
-  apply (simp add: cval_def gval.simps ValueGt_def)
-  apply (rule allI)
-  apply (case_tac r)
-     apply (simp add: gval.simps)
-    apply (case_tac x2)
-  by (simp_all add: gval.simps ValueEq_def)
+  apply (rule observe_trace_possible_step)
+     apply (simp add: possible_steps_0)
+    apply (simp add: select_def)
+   apply simp
+  apply (rule observe_trace_possible_step)
+     apply (simp add: possible_steps_1)
+    apply (simp add: coin_def apply_outputs select_def)
+   apply simp
+  apply (rule observe_trace_possible_step)
+     apply (simp add: possible_steps_2_coin)
+    apply (simp add: coin_def apply_outputs select_def)
+   apply simp
+  apply (rule observe_trace_possible_step)
+     apply simp
+     apply (rule possible_steps_2_vend)
+      apply (simp add: coin_def select_def join_ir_def input2state_def)
+     apply simp
+    apply (simp add: vend_def apply_outputs)
+    apply (simp add: coin_def select_def)
+   apply simp
+  by simp
 
 lemma drinks2_0_invalid: "\<not> (aa = (STR ''select'') \<and> length (b) = 1) \<Longrightarrow>
     (possible_steps drinks2 0 Map.empty aa b) = {||}"
   apply (simp add: drinks2_def possible_steps_def transitions)
   by force
 
-lemma step_0: "length i = 1 \<Longrightarrow> step drinks2 0 Map.empty (STR ''select'') i = Some (select, 1, [], <R 1 := hd i, R 2 := Num 0>)"
+lemma step_0: "length i = 1 \<Longrightarrow> step drinks2 0 Map.empty (STR ''select'') i = Some (select, 1, [], <1 := hd i, 2 := Num 0>)"
   apply (simp add: step_def possible_steps_0 select_def)
   apply (rule ext)
-  apply (simp)
-  using hd_input2state by auto
-
-lemma updates_select: "length (snd a) = 1 \<Longrightarrow> (EFSM.apply_updates (Updates select) (case_vname (\<lambda>n. input2state (snd a) 1 (I n)) Map.empty) Map.empty) = <R 1:=hd (snd a), R 2 := Num 0>"
-  apply (simp add: select_def)
-  apply (rule ext)
-  by (simp add: hd_input2state)
+  apply (simp add: join_ir_def input2state_nth)
+  by (metis hd_conv_nth list.size(3) zero_neq_one)
 
 lemma drinks2_vend_empty: "possible_steps drinks2 0 Map.empty ((STR ''vend'')) [] = {||}"
   using drinks2_0_invalid by auto
@@ -201,89 +101,30 @@ lemma drinks2_vend_insufficient: "possible_steps drinks2 1 r ((STR ''vend'')) []
   apply (simp add: possible_steps_def drinks2_def transitions)
   by force
 
-lemma apply_updates_vend_fail: "(EFSM.apply_updates (Updates vend_fail) (case_vname Map.empty (\<lambda>n. if n = 2 then Some (Num n') else <R 1 := s> (R n)))
-         <R 1 := s, R 2 := Num 0>) = <R 1 := s, R 2 := Num n'>"
-  apply (rule ext)
-  by (simp add: vend_fail_def)
-
-lemma apply_updates_vend_nothing: "(EFSM.apply_updates (Updates vend_nothing) (case_vname Map.empty (\<lambda>n. if n = 2 then Some (Num n') else <R 1 := s> (R n)))
-         <R 1 := s, R 2 := Num 0>) = <R 1 := s, R 2 := Num n'>"
-  apply (rule ext)
-  by (simp add: vend_nothing_def)
-
-lemma coin_updates: "(EFSM.apply_updates (Updates coin) (case_vname (\<lambda>n. input2state (snd a) 1 (I n)) (\<lambda>n. if n = 2 then Some v else if R n = R 1 then Some s else None))
-       (\<lambda>a. if a = R 2 then Some v else if a = R 1 then Some s else None)) = (\<lambda>u. if u = R 1 then Some s else if u = R 2 then value_plus (Some v) (input2state (snd a) 1 (I 1)) else None)"
-  apply (rule ext)
-  by (simp add: coin_def)
-
 lemma drinks2_2_coin: "fst a = (STR ''coin'') \<and> length (snd a) = 1 \<Longrightarrow> possible_steps drinks2 2 r ((STR ''coin'')) (snd a) = {|(2, coin)|}"
   unfolding possible_steps_def
   apply (simp add: possible_steps_def drinks2_def transitions)
   by force
 
-lemma updates_coin_2: "(EFSM.apply_updates (Updates coin) (case_vname (\<lambda>n. input2state (snd a) 1 (I n)) (\<lambda>n. if n = 1 then Some s else if R n = R 2 then r2 else None))
-             (\<lambda>u. if u = R 1 then Some s else if u = R 2 then r2 else None)) = (\<lambda>u. if u = R 1 then Some s else if u = R 2 then value_plus r2  (input2state (snd a) 1 (I 1)) else None)"
-  apply (rule ext)
-  by (simp add: coin_def)
-
-lemma drinks2_vend_r2_none: "r (R 2) = None \<Longrightarrow> possible_steps drinks2 2 r ((STR ''vend'')) [] = {||}"
-  apply (simp add: possible_steps_def ffilter_def fset_both_sides Abs_fset_inverse drinks2_def Set.filter_def)
-  apply (rule allI)+
-  apply (case_tac "ba = coin")
-   apply (simp add: coin_def)
-  apply (case_tac "ba = vend_fail")
-   apply (simp add: transitions gval.simps ValueGt_def)
-  by (simp add: transitions gval.simps ValueGt_def)
+lemma drinks2_vend_r2_none: "r 2 = None \<Longrightarrow> possible_steps drinks2 2 r ((STR ''vend'')) [] = {||}"
+  apply (simp add: possible_steps_empty drinks2_def)
+  apply safe
+  by (simp_all add: transitions apply_guards_def ValueGt_def join_ir_def)
 
 lemma label_vend_not_coin: "Label b = ((STR ''vend'')) \<Longrightarrow> b \<noteq> coin"
   using label_coin by auto
 
-lemma drinks2_vend_insufficient2: "r (R 2) = Some (Num x1) \<and> x1 < 100 \<Longrightarrow> possible_steps drinks2 2 r ((STR ''vend'')) [] = {|(2, vend_fail)|}"
-proof-
-  assume premise: "r (R 2) = Some (Num x1) \<and> x1 < 100"
-  have filter: "ffilter
-     (\<lambda>((origin, dest), t).
-         origin = 2 \<and>
-         Label t = STR ''vend'' \<and> Arity t = 0 \<and> apply_guards (Guard t) (\<lambda>x. case x of I n \<Rightarrow> input2state [] 1 (I n) | R n \<Rightarrow> r (R n)))
-     drinks2 =
-    {|((2, 2), vend_fail)|}"
-    using premise
-    apply (simp add: ffilter_def fset_both_sides Abs_fset_inverse Set.filter_def drinks2_def)
-    apply safe
-    by (simp_all add: transitions gval.simps ValueGt_def)
-  show ?thesis
-    by (simp add: possible_steps_def filter)
-qed
+lemma drinks2_vend_insufficient2: "r 2 = Some (Num x1) \<and> x1 < 100 \<Longrightarrow> possible_steps drinks2 2 r ((STR ''vend'')) [] = {|(2, vend_fail)|}"
+  apply (simp add: possible_steps_singleton drinks2_def)
+  apply safe
+  by (simp_all add: transitions apply_guards_def ValueGt_def)
 
-lemma updates_vend_fail: "(EFSM.apply_updates (Updates vend_fail) (case_vname Map.empty (\<lambda>n. if n = 1 then Some s else if R n = R 2 then r2 else None))
-                   (\<lambda>u. if u = R 1 then Some s else if u = R 2 then r2 else None)) = (\<lambda>u. if u = R 1 then Some s else if u = R 2 then r2 else None)"
-  apply (rule ext)
-  by (simp add: vend_fail_def)
-
-lemma drinks2_vend_sufficient: "r (R 2) = Some (Num x1) \<Longrightarrow>
+lemma drinks2_vend_sufficient: "r 2 = Some (Num x1) \<Longrightarrow>
                 \<not> x1 < 100 \<Longrightarrow>
                 possible_steps drinks2 2 r ((STR ''vend'')) [] = {|(3, vend)|}"
-proof-
-  assume premise1: "r (R 2) = Some (Num x1)"
-  assume premise2 : "\<not> x1 < 100"
-  have filter: "ffilter
-     (\<lambda>((origin, dest), t).
-         origin = 2 \<and>
-         Label t = STR ''vend'' \<and> Arity t = 0 \<and> apply_guards (Guard t) (\<lambda>x. case x of I n \<Rightarrow> input2state [] 1 (I n) | R n \<Rightarrow> r (R n)))
-     drinks2 =
-    {|((2, 3), vend)|}"
-    using premise1 premise2
-    apply (simp add: ffilter_def fset_both_sides Abs_fset_inverse Set.filter_def drinks2_def)
-    apply safe
-    by (simp_all add: transitions gval.simps ValueGt_def)
-  show ?thesis
-    by (simp add: possible_steps_def filter)
-qed
-
-lemma vend_updates: "(EFSM.apply_updates (Updates vend) (case_vname Map.empty (\<lambda>n. if n = 1 then Some s else if R n = R 2 then r2 else None))
-                   (\<lambda>u. if u = R 1 then Some s else if u = R 2 then r2 else None)) = (\<lambda>u. if u = R 1 then Some s else if u = R 2 then r2 else None)"
-  apply (rule ext)
-  by (simp add: vend_def)
+  apply (simp add: possible_steps_singleton drinks2_def)
+  apply safe
+  by (simp_all add: transitions apply_guards_def ValueGt_def)
 
 lemma drinks2_end: "possible_steps drinks2 3 r a b = {||}"
   apply (simp add: possible_steps_def drinks2_def transitions)
@@ -299,15 +140,11 @@ next
     by (simp add: observe_trace_def step_def drinks2_end drinks_end )
 qed
 
-lemma drinks2_vend_r2_String: "r (R 2) = Some (value.Str x2) \<Longrightarrow>
+lemma drinks2_vend_r2_String: "r 2 = Some (value.Str x2) \<Longrightarrow>
                 possible_steps drinks2 2 r ((STR ''vend'')) [] = {||}"
-  apply (simp add: possible_steps_def ffilter_def fset_both_sides Abs_fset_inverse Set.filter_def drinks2_def)
-  apply (rule allI)+
-  apply (case_tac "ba = coin")
-   apply (simp add: coin_def)
-  apply (case_tac "ba = vend_fail")
-   apply (simp add: vend_fail_def gval.simps ValueGt_def)
-  by (simp add: vend_def gval.simps ValueGt_def)
+  apply (simp add: possible_steps_empty drinks2_def)
+  apply safe
+  by (simp_all add: transitions apply_guards_def ValueGt_def join_ir_def)
 
 lemma drinks2_2_invalid: "fst a = (STR ''coin'') \<longrightarrow> length (snd a) \<noteq> 1 \<Longrightarrow>
           a \<noteq> ((STR ''vend''), []) \<Longrightarrow>
@@ -319,201 +156,123 @@ lemma drinks2_2_invalid: "fst a = (STR ''coin'') \<longrightarrow> length (snd a
   apply simp
   by (metis length_0_conv prod.collapse select_convs(1) select_convs(2))
 
-lemma equal_1_2: "\<forall>r2. observe_trace drinks 1 (\<lambda>u. if u = R 1 then Some s else if u = R 2 then r2 else None) t =
-    observe_trace drinks2 2 (\<lambda>u. if u = R 1 then Some s else if u = R 2 then r2 else None) t"
-proof (induction t)
-  case Nil
-  then show ?case
-    by (simp add: observe_trace_def)
-next
-  case (Cons a t)
-  then show ?case
-    apply clarify
-    apply (case_tac "fst a = (STR ''coin'') \<and> length (snd a) = 1")
-    unfolding observe_trace_def
-    apply (simp add: step_def)
-     apply (simp add: drinks_1_coin coin_updates drinks2_2_coin updates_coin_2)
-     apply (simp)
-
-    apply (simp add: step_def)
-    apply (case_tac "a = ((STR ''vend''), [])")
-     apply (case_tac r2)
-      apply (simp add: step_def)
-    apply (simp add: drinks_vend_r2_none drinks2_vend_r2_none )
-     apply (case_tac aa)
-      apply (case_tac "x1 < 100")
-    apply (simp add: step_def)
-    apply (simp add: drinks_vend_insufficient drinks2_vend_insufficient2 updates_vend_fail )
-    apply (simp add: step_def)
-      apply (simp add: drinks_vend_sufficient drinks2_vend_sufficient vend_updates )
-    using equal_2_3 observe_trace_def apply auto[1]
-     apply (simp add: step_def)
-     apply (simp add: drinks_vend_r2_String drinks2_vend_r2_String )
-    by (simp add: drinks_1_inaccepts drinks2_2_invalid )
-qed
-
 lemma drinks2_1_invalid: "\<not>(a = (STR ''coin'') \<and> length b = 1) \<Longrightarrow>
       \<not>(a = (STR ''vend'') \<and> b = []) \<Longrightarrow>
     possible_steps drinks2 1 r a b = {||}"
-proof-
-  assume premise1: "\<not>(a = (STR ''coin'') \<and> length b = 1)"
-  assume premise2: "\<not>(a = (STR ''vend'') \<and> b = [])"
-  have set_filter: "Set.filter
-       (\<lambda>((origin, dest), t).
-           origin = 1 \<and> Label t = a \<and> length b = Arity t \<and> apply_guards (Guard t) (case_vname (\<lambda>n. input2state b 1 (I n)) (\<lambda>n. r (R n))))
-       (fset drinks2) = {}"
-    using premise1 premise2
-    apply (simp add: Set.filter_def drinks2_def)
-    apply safe
-    by (simp_all add: transitions)
-  show ?thesis
-    by (simp add: possible_steps_def ffilter_def set_filter)
-qed
+  apply (simp add: possible_steps_empty drinks2_def)
+  apply safe
+  by (simp_all add: transitions apply_guards_def ValueGt_def join_ir_def)
 
-lemma coin_updates_equiv: "(EFSM.apply_updates (Updates coin)
-         (case_vname (\<lambda>n. input2state (snd a) 1 (I n)) (\<lambda>n. if n = 2 then Some (Num 0) else <R 1 := s> (R n)))
-         <R 1 := s, R 2 := Num 0>) = (\<lambda>u. if u = R 1 then Some s else if u = R 2 then value_plus (Some (Num 0)) (input2state (snd a) 1 (I 1))
- else None)"
-  apply (simp add: coin_def)
+lemma apply_updates_select: "length (snd a) = 1 \<Longrightarrow> apply_updates (Updates select) (join_ir (snd a) Map.empty) Map.empty = <1 := hd (snd a), 2 := Num 0>"
   apply (rule ext)
-  by simp
+  apply (simp add: apply_updates_def select_def join_ir_def input2state_nth)
+  by (metis hd_conv_nth list.size(3) zero_neq_one)
 
-lemma equal_1_1: "observe_trace drinks 1 <R 1 := s, R 2 := Num 0> t = observe_trace drinks2 1 <R 1 := s, R 2 := Num 0> t"
-proof (induction t)
+lemma apply_updates_vend_fail: "apply_updates (Updates vend_fail) (join_ir i r) r = r"
+  apply (rule ext)
+  by (simp add: transitions join_ir_def)
+
+lemma apply_updates_vend_nothing: "apply_updates (Updates vend_nothing) (join_ir i r) r = r"
+  apply (rule ext)
+  by (simp add: transitions join_ir_def)
+
+lemma drinks2_vend_invalid: "\<nexists>n. r 2 = Some (Num n) \<Longrightarrow> possible_steps drinks2 2 r (STR ''vend'') [] = {||}"
+  apply (simp add: possible_steps_empty drinks2_def)
+  apply safe
+  by (simp_all add: transitions apply_guards_def join_ir_def ValueGt_def MaybeBoolInt_not_num_1)
+
+lemma equal_1_2: "\<forall>r. observe_trace drinks 1 r t = observe_trace drinks2 2 r t"
+  apply clarify
+proof(induct t)
   case Nil
   then show ?case
-    unfolding observe_trace_def
     by simp
 next
   case (Cons a t)
   then show ?case
-    unfolding observe_trace_def
     apply (case_tac "fst a = (STR ''coin'') \<and> length (snd a) = 1")
-     apply (simp add: step_def)
-     apply (simp only: drinks_1_coin possible_steps_1)
-     apply (simp add: )
-    apply (simp only: coin_updates_equiv)
-    using equal_1_2 observe_trace_def
-    apply simp
-    apply (case_tac "a = ((STR ''vend''), [])")
-      apply (simp)
-      apply (simp add: step_def drinks_vend_insufficient drinks2_vend_insufficient)
-     apply (simp add: outputs_vend_fail outputs_vend_nothing )
-     apply (simp add: apply_updates_vend_fail apply_updates_vend_nothing)
-
-    apply (case_tac a)
-    apply (simp add: step_def)
-    using drinks_1_inaccepts drinks2_1_invalid step_def
+     defer
+     apply (case_tac "a = (STR ''vend'', [])")
+      prefer 2
+      apply (rule efsm_equiv_no_possible_step)
+       apply (simp add: drinks_1_inaccepts)
+    using drinks2_2_invalid apply blast
+     apply (case_tac "r 2")
+      apply (rule efsm_equiv_no_possible_step)
+       apply (simp add: drinks_vend_invalid)
+      apply (simp add: drinks2_vend_invalid)
+     apply (case_tac aa)
+      prefer 2
+      apply (rule efsm_equiv_no_possible_step)
+       apply (simp add: drinks_vend_invalid)
+      apply (simp add: drinks2_vend_invalid)
+     apply (case_tac "x1 \<ge> 100")
+      apply (rule efsm_equiv_possible_step)
+           apply (simp add: Drinks_Machine.possible_steps_2_vend)
+          apply (simp add: possible_steps_2_vend)
+         apply simp
+        apply simp
+       apply simp
+      apply (simp add: equal_2_3)
+     apply (rule efsm_equiv_possible_step)
+          apply (simp add: drinks_vend_insufficient)
+         apply (simp add: not_le drinks2_vend_insufficient2)
+        apply simp+
+    apply (rule efsm_equiv_possible_step)
+         apply (simp add: Drinks_Machine.possible_steps_1_coin)
+        apply (simp add: possible_steps_2_coin)
     by auto
 qed
 
-lemma observational_equivalence: "efsm_equiv drinks drinks2 t" (* Corresponds to Example 3 in Foster et. al. *)
+lemma eq_1_1: "observe_trace drinks 1 <1 := d, 2 := Num 0> t = observe_trace drinks2 1 <1 := d, 2 := Num 0> t"
+proof(induct t)
+    case Nil
+    then show ?case
+      by simp
+  next
+    case (Cons a1 t1)
+    then show ?case
+      apply (case_tac "fst a1 = (STR ''coin'') \<and> length (snd a1) = 1")
+       defer
+       apply (case_tac "a1 = (STR ''vend'', [])")
+        prefer 2
+        apply (rule efsm_equiv_no_possible_step)
+         apply (simp add: drinks_1_inaccepts)
+        apply (metis drinks2_1_invalid prod.collapse)
+       apply (rule efsm_equiv_possible_step)
+            apply (simp add: drinks_vend_insufficient)
+           apply (simp add: drinks2_vend_insufficient)
+          apply (simp add: transitions)
+         apply simp
+        apply simp
+       apply (simp add: apply_updates_vend_fail apply_updates_vend_nothing)
+      apply (rule efsm_equiv_possible_step)
+           apply (simp add:possible_steps_1_coin)
+          apply (simp add: possible_steps_1)
+         apply simp
+        apply simp
+       apply simp
+      by (simp add: equal_1_2)
+  qed
+
+(* Corresponds to Example 3 in Foster et. al. *)
+lemma observational_equivalence: "efsm_equiv drinks drinks2 t"
 proof (induct t)
   case Nil
     then show ?case by (simp add: efsm_equiv_def observe_trace_def)
   next
   case (Cons a t)
   then show ?case
-    apply (simp only: efsm_equiv_def observe_trace_def)
+    apply (simp only: efsm_equiv_def)
     apply (case_tac "fst a = (STR ''select'') \<and> length (snd a) = 1")
      prefer 2
-     apply (simp add: drinks2_0_invalid drinks_0_inaccepts is_singleton_def step_def )
-    apply (simp)
-    apply (simp add: possible_steps_0 Drinks_Machine.possible_steps_0 updates_select step_def)
-    apply (case_tac t)
-     apply simp
-    using equal_1_1
-    by (metis observe_trace_def)
-qed
-
-lemma step_drinks_2: "step drinks2 0 Map.empty aa ba = Some (uw, s', ux, r') \<Longrightarrow> (uw, s', ux, r') = (select, 1, [], <R 1 := hd ba, R 2 := Num 0>)"
-  apply (simp add: step_def)
-  apply (case_tac "aa = (STR ''select'') \<and> length ba = 1")
-   apply (simp add: possible_steps_0)
-   apply clarify
-   apply (simp add: select_def)
-   apply (rule ext)
-   apply (simp add: hd_input2state)
-  by (simp add: drinks2_0_invalid)
-
-lemma step_drinks2_vend_fail: "step drinks2 1 ra (STR ''vend'') [] = Some (vend_nothing, 1, [], ra)"
-  apply (simp add: step_def drinks2_vend_insufficient)
-  apply (simp add: vend_nothing_def)
-  apply (rule ext)
-  by simp
-
-lemma step_2_or_3: "step drinks2 2 r a b = Some (uw, s', ux, r') \<Longrightarrow> s' = 2 \<or> s' = 3"
-  apply (simp add: step_def)
-  apply (case_tac "a = (STR ''coin'') \<and> length b = 1")
-   apply simp
-  using drinks2_2_coin
-   apply auto[1]
-  apply simp
-  apply (case_tac "a = (STR ''vend'') \<and> b = []")
-   apply simp
-   apply clarify
-   apply (case_tac "r (R 2)")
-    apply (simp add: drinks2_vend_r2_none)
-   apply (case_tac aa)
-    prefer 2
-    apply (simp add: drinks2_vend_r2_String)
-   apply simp
-   apply (case_tac "x1 < 100")
-    apply (simp add: drinks2_vend_insufficient2)
-    apply (simp add: drinks2_vend_sufficient)
-  using drinks2_2_invalid
-  by auto
-
-lemma no_route_from_3_to_1: "\<forall>r. \<not> gets_us_to 1 drinks2 3 r lst"
-proof (induct lst)
-  case Nil
-  then show ?case
-    apply safe
-    apply (rule gets_us_to.cases)
-    by auto
-next
-  case (Cons a lst)
-  then show ?case
-    apply safe
-    apply (rule gets_us_to.cases)
-       apply simp
-      apply simp
-     apply simp
-     apply clarify
-     apply simp
-     apply (simp add: step_def)
-    using drinks2_end
-     apply auto[1]
-    by simp
-qed
-
-lemma no_route_from_2_to_1: "\<forall>r. \<not> gets_us_to 1 drinks2 2 r lst"
-proof (induct lst)
-  case Nil
-  then show ?case
-    apply safe
-    apply (rule gets_us_to.cases)
-    by auto
-next
-  case (Cons a lst)
-  then show ?case
-    apply safe
-    apply (rule gets_us_to.cases)
-       apply simp
-      apply simp
-    defer
-     apply simp
-    apply simp
-    apply clarify
-    apply simp
-    apply (case_tac "s'=2")
-    apply simp
-    apply (case_tac "s'=3")
-    defer
-    using step_2_or_3
-     apply blast
-    apply simp
-    using no_route_from_3_to_1
-    by simp
+     apply (rule efsm_equiv_no_possible_step)
+    using drinks_0_inaccepts apply blast
+    using drinks2_0_invalid apply simp
+    apply (rule efsm_equiv_possible_step)
+         apply (simp add: Drinks_Machine.possible_steps_0)
+        apply (simp add: possible_steps_0)
+       apply simp+
+    by (simp only: apply_updates_select eq_1_1)
 qed
 end
